theories/coneris/lib/flip.v
@@ -103,17 +103,19 @@ Section specs.
     intros n; inv_fin n.
   Qed.
 
-  Lemma awp_flip_adv E (ε:nonnegreal) ε2 : 
-    (nonneg ε = 1/2 * (nonneg (ε2 true) + nonneg (ε2 false)))%R -> ⊢
-    (<<{ ↯ ε }>> flip @ E <<{ ∃∃ (b:bool), ↯ (ε2 b) | RET #b }>>)%I.
+  Lemma awp_flip_adv E (ε2 : nonnegreal -> bool -> nonnegreal):
+    (∀ ε, nonneg ε = 1/2 * (nonneg (ε2 ε true) + nonneg (ε2 ε false)))%R ->
+    ⊢(<<{ ∀∀ (ε:nonnegreal), ↯ ε }>> flip @ E
+       <<{ ∃∃ (b:bool) ,
+             ↯ (ε2 ε b) | RET #b }>>)%I.
   Proof.
-    iIntros (??) "AU".
+    iIntros (K ?) "AU".
     rewrite /flip/flipL.
     wp_pures.
     wp_bind (rand _)%E.
-    iMod "AU" as "[Herr [_ Hclose]]".
-    wp_apply (wp_couple_rand_adv_comp1 _ _ _ _ (λ x, if fin_to_nat x =? 0%nat then ε2 false else ε2 true) with "[$Herr]").
-    { rewrite SeriesC_finite_foldr. simpl. lra. }
+    iMod "AU" as "[%ε [Herr [_ Hclose]]]".
+    wp_apply (wp_couple_rand_adv_comp1 _ _ _ _ (λ x, if fin_to_nat x =? 0%nat then ε2 ε false else ε2 ε true) with "[$Herr]").
+    { rewrite SeriesC_finite_foldr. simpl. rewrite (K ε). lra. }
     iIntros (n) "? /=".
     inv_fin n; simpl; [|intros n; inv_fin n; simpl; [|intros n; inv_fin n]].
     all: iMod ("Hclose" with "[$]"); iModIntro; wp_apply (wp_int_to_bool with "[//]").
